heap.v
@@ -1,0 +1,319 @@
+From lrust Require Export lifting.
+From iris.algebra Require Import upred_big_op cmra_big_op frac dec_agree csum.
+From iris.program_logic Require Export invariants ghost_ownership.
+From iris.program_logic Require Import ownership auth.
+From iris.proofmode Require Import weakestpre invariants.
+Import uPred.
+
+Definition lock_stateR : cmraT := csumR (exclR unitC) natR.
+
+Definition heapValUR : ucmraT :=
+  gmapUR loc (prodR (prodR fracR lock_stateR) (dec_agreeR val)).
+
+Definition heapFreeUR : ucmraT :=
+  gmapUR block (prodR fracR (gmapR Z (exclR unitC))).
+
+Class heapG Σ := HeapG {
+  heapVal_inG :> authG lrust_lang Σ heapValUR;
+  heapFree_inG :> authG lrust_lang Σ heapFreeUR;
+  heapVal_name : gname;
+  heapFree_name : gname
+}.
+Definition heapValGF : gFunctor := authGF heapValUR.
+Definition heapFreeGF : gFunctor := authGF heapFreeUR.
+
+Definition of_lock_state (x : lock_state) : lock_stateR :=
+  match x with
+  | RSt n => Cinr n
+  | WSt => Cinl (Excl ())
+  end.
+Definition to_heapVal : state → heapValUR :=
+  fmap (λ v, (1%Qp, of_lock_state (v.1), DecAgree (v.2))).
+Definition heapFree_rel (σ : state) (heapFree : heapFreeUR) : Prop :=
+  ∀ blk q s, heapFree !! blk = Some(q, s) →
+  s ≠ ∅ ∧ ∀ i, is_Some (σ !! (blk, i)) ↔ is_Some (s !! i).
+
+Section definitions.
+  Context `{i : heapG Σ}.
+
+  Definition heap_mapsto_def (l : loc) (q : Qp) (v: val) : iPropG lrust_lang Σ :=
+    auth_own heapVal_name {[ l := (q, Cinr O, DecAgree v) ]}.
+  Definition heap_mapsto_aux : { x | x = @heap_mapsto_def }. by eexists. Qed.
+  Definition heap_mapsto := proj1_sig heap_mapsto_aux.
+  Definition heap_mapsto_eq : @heap_mapsto = @heap_mapsto_def :=
+    proj2_sig heap_mapsto_aux.
+
+  Definition heap_mapsto_vec (l : loc) (q : Qp) (vl : list val) :
+    iPropG lrust_lang Σ :=
+    ([★] imap (fun i v => heap_mapsto (shift_loc l i) q v) vl)%I.
+
+  Fixpoint inter (i0 : Z) (n : nat) : gmapR Z (exclR unitC) :=
+    match n with
+    | O => ∅
+    | S n => <[i0 := Excl ()]>(inter (i0+1) n)
+    end.
+  Definition heap_freeable_def (l : loc) (q : Qp) (n: nat) : iPropG lrust_lang Σ :=
+    auth_own heapFree_name {[ l.1 := (q, inter (l.2) n) ]}.
+  Definition heap_freeable_aux : { x | x = @heap_freeable_def }. by eexists. Qed.
+  Definition heap_freeable := proj1_sig heap_freeable_aux.
+  Definition heap_freeable_eq : @heap_freeable = @heap_freeable_def :=
+    proj2_sig heap_freeable_aux.
+
+  Definition heap_inv : iPropG lrust_lang Σ :=
+    (∃ σ heapFree, ownP σ ★ own heapVal_name (● to_heapVal σ)
+               ★ own heapFree_name (● heapFree) ★ ■ heapFree_rel σ heapFree)%I.
+  Definition heap_ctx (N : namespace) := inv N heap_inv.
+
+  Global Instance heap_ctx_persistent N : PersistentP (heap_ctx N).
+  Proof. apply _. Qed.
+End definitions.
+
+Typeclasses Opaque heap_ctx heap_mapsto heap_freeable.
+Instance: Params (@heap_mapsto) 4.
+Instance: Params (@heap_freeable) 5.
+Instance: Params (@heap_ctx) 2.
+
+Notation "l ↦{ q } v" := (heap_mapsto l q v)
+  (at level 20, q at level 50, format "l ↦{ q } v") : uPred_scope.
+Notation "l ↦ v" := (heap_mapsto l 1 v) (at level 20) : uPred_scope.
+
+Notation "l ↦★{ q } vl" := (heap_mapsto_vec l q vl)
+  (at level 20, q at level 50, format "l ↦★{ q }  vl") : uPred_scope.
+Notation "l ↦★ vl" := (heap_mapsto_vec l 1 vl) (at level 20) : uPred_scope.
+
+Notation "†{ q } l … n" := (heap_freeable l q n)
+  (at level 20, q at level 50, format "†{ q } l … n") : uPred_scope.
+Notation "† l … n" := (heap_freeable l 1 n) (at level 20) : uPred_scope.
+
+Section heap.
+  Context {Σ : gFunctors}.
+  Implicit Types N : namespace.
+  Implicit Types P Q : iPropG lrust_lang Σ.
+  Implicit Types Φ : val → iPropG lrust_lang Σ.
+  Implicit Types σ : state.
+
+  (** Allocation *)
+  Lemma to_heap_valid σ : ✓ to_heapVal σ.
+  Proof. intros l. rewrite lookup_fmap. case (σ !! l)=>[[[|n] v]|]//=. Qed.
+  Lemma heap_alloc N E σ :
+    authG lrust_lang Σ heapValUR → authG lrust_lang Σ heapFreeUR →
+    nclose N ⊆ E →
+    ownP σ ={E}=> ∃ _ : heapG Σ, heap_ctx N.
+  Proof.
+    iIntros {???} "Hσ".
+    iPvs (own_alloc (● to_heapVal σ)) as {vγ} "Hvγ".
+    { split; last apply to_heap_valid. intro. apply ucmra_unit_leastN. }
+    iPvs (own_alloc (● (∅ : heapFreeUR))) as {fγ} "Hfγ".
+    { split. intro. apply ucmra_unit_leastN. apply ucmra_unit_valid. }
+    set (HeapG _ _ _ vγ fγ). unfold heap_ctx. iExists _.
+    iPvs (inv_alloc N E heap_inv with "[-]") as "HN"; try done.
+    iNext. iExists _, _. iFrame. iPureIntro. intros ???. by rewrite lookup_empty.
+  Qed.
+
+  Context `{heapG Σ}.
+
+  (** General properties of mapsto *)
+  Global Instance heap_mapsto_timeless l q v : TimelessP (l↦{q}v).
+  Proof. rewrite heap_mapsto_eq /heap_mapsto_def. apply _. Qed.
+
+  Global Instance heap_mapsto_vec_timeless l q vl : TimelessP (l ↦★{q} vl).
+  Proof.
+    unfold heap_mapsto_vec, imap. generalize O. induction vl=>/=; apply _.
+  Qed.
+
+  Lemma heap_mapsto_op_eq l q1 q2 v : l ↦{q1} v ★ l ↦{q2} v ⊣⊢ l ↦{q1+q2} v.
+  Proof.
+    by rewrite heap_mapsto_eq -auth_own_op op_singleton pair_op dec_agree_idemp.
+  Qed.
+
+  Lemma heap_mapsto_vec_op_eq l q1 q2 vl :
+    l ↦★{q1} vl ★ l ↦★{q2} vl ⊣⊢ l ↦★{q1+q2} vl.
+  Proof.
+    unfold heap_mapsto_vec, imap. generalize O. induction vl as [|v vl IH]=>/= n.
+    - apply right_id, _.
+    - rewrite -IH -heap_mapsto_op_eq equiv_spec.
+      by split; iIntros "[[??][??]]"; iFrame.
+  Qed.
+
+  Lemma heap_mapsto_op l q1 q2 v1 v2 :
+    l ↦{q1} v1 ★ l ↦{q2} v2 ⊣⊢ v1 = v2 ∧ l ↦{q1+q2} v1.
+  Proof.
+    destruct (decide (v1 = v2)) as [->|].
+    { by rewrite heap_mapsto_op_eq pure_equiv // left_id. }
+    rewrite heap_mapsto_eq -auth_own_op op_singleton pair_op dec_agree_ne //.
+    apply (anti_symm (⊢)); last by apply pure_elim_l.
+    rewrite auth_own_valid gmap_validI (forall_elim l) lookup_singleton.
+    rewrite option_validI prod_validI !discrete_valid. by apply pure_elim_r.
+  Qed.
+
+  Lemma heap_mapsto_vec_op l q1 q2 vl1 vl2 :
+    length vl1 = length vl2 →
+    l ↦★{q1} vl1 ★ l ↦★{q2} vl2 ⊣⊢ vl1 = vl2 ∧ l ↦★{q1+q2} vl1.
+  Proof.
+    unfold heap_mapsto_vec, imap. generalize O. revert vl2.
+    induction vl1 as [|v1 vl1 IH]=>[][|v2 vl2]n/=; try done.
+    - rewrite equiv_spec. split; iIntros; auto.
+    - assert (∀ A B C D : iPropG lrust_lang Σ,
+                 (A ★ B) ★ (C ★ D) ⊣⊢ (A ★ C) ★ (B ★ D)) as ->.
+      { by intros; rewrite equiv_spec; split; iIntros "[[??][??]]"; iFrame. }
+      intros [=?]. rewrite heap_mapsto_op IH // equiv_spec; split.
+      + iIntros "[[%?][%?]]". subst. iSplit. auto. by iFrame.
+      + iIntros "[#Heq[Hv Hvl]]". iDestruct "Heq" as %[=->->]. iSplitL "Hv"; auto.
+  Qed.
+
+  Lemma heap_mapsto_vec_app_op l q vl1 vl2 :
+    l ↦★{q} vl1 ★ (shift_loc l (length vl1)) ↦★{q} vl2 ⊣⊢ l ↦★{q} (vl1++vl2).
+  Proof.
+    unfold heap_mapsto_vec, imap. generalize O. induction vl1 as [|v1 vl1 IH]=>n/=.
+    - by rewrite left_id shift_loc_0.
+    - rewrite -IH assoc. f_equiv. clear IH. revert n.
+      induction vl2 as [|v2 vl2 IH]=>n //=.
+      rewrite !shift_loc_assoc IH. apply reflexive_eq. repeat (lia||f_equal).
+  Qed.
+
+  Lemma heap_mapsto_op_split l q v : l ↦{q} v ⊣⊢ (l ↦{q/2} v ★ l ↦{q/2} v).
+  Proof. by rewrite heap_mapsto_op_eq Qp_div_2. Qed.
+
+  Lemma heap_mapsto_vec_op_split l q vl :
+    l ↦★{q} vl ⊣⊢ (l ↦★{q/2} vl ★ l ↦★{q/2} vl).
+  Proof. by rewrite heap_mapsto_vec_op_eq Qp_div_2. Qed.
+
+  Lemma heap_mapsto_vec_auth l q vl:
+    vl ≠ [] →
+    l ↦★{q} vl ⊣⊢
+      auth_own heapVal_name (big_op (imap
+        (λ i v, {[shift_loc l i := (q, Cinr 0%nat, DecAgree v)]}) vl)).
+  Proof.
+    rewrite /heap_mapsto_vec heap_mapsto_eq /heap_mapsto_def.
+    revert l. induction vl as [|v vl IH]=>// l _. destruct (decide (vl = [])).
+    - subst. simpl. by rewrite !right_id.
+    - rewrite !imap_cons auth_own_op /=.
+      erewrite imap_ext, (IH (shift_loc l 1)), imap_ext; [done| |done|];
+        simpl; intros i v'; rewrite shift_loc_assoc; repeat f_equiv; lia.
+  Qed.
+
+  Lemma inter_lookup_Some i j (n:nat):
+    i ≤ j < i+n → inter i n !! j = Excl' ().
+  Proof.
+    revert i. induction n=>/= i. lia. rewrite lookup_insert_Some.
+    destruct (decide (i = j)); naive_solver lia.
+  Qed.
+  Lemma inter_lookup_None i j (n : nat):
+    j < i ∨ i+n ≤ j → inter i n !! j = None.
+  Proof.
+    revert i. induction n=>/= i. by rewrite lookup_empty.
+    rewrite lookup_insert_None. naive_solver lia.
+  Qed.
+  Lemma inter_op i n n': inter i n ⋅ inter (i+n) n' ≡ inter i (n+n').
+  Proof.
+    intro j. rewrite lookup_op.
+    destruct (decide (i ≤ j < i+n)); last destruct (decide (i+n ≤ j < i+n+n')).
+    - by rewrite (inter_lookup_None (i+n) j n') ?inter_lookup_Some; try lia.
+    - by rewrite (inter_lookup_None i j n) ?inter_lookup_Some; try lia.
+    - by rewrite !inter_lookup_None; try lia.
+  Qed.
+  Lemma inter_valid i n : ✓ inter i n.
+  Proof. revert i. induction n=>i. done. by apply insert_valid. Qed.
+
+  Lemma heap_freeable_op_eq l q1 q2 n n' :
+    †{q1}l…n ★ †{q2}(shift_loc l n)…n' ⊣⊢ †{q1+q2}(l)…(n+n').
+  Proof.
+    by rewrite heap_freeable_eq /heap_freeable_def -auth_own_op op_singleton
+               pair_op inter_op.
+  Qed.
+
+  (** Weakest precondition *)
+  Lemma init_mem_update_val σ l vl:
+    (∀ m : Z, σ !! shift_loc l m = None) →
+    ● to_heapVal σ ~~> ● to_heapVal (init_mem l vl σ)
+      ⋅ ◯ big_op (imap
+            (λ i v, {[shift_loc l i := (1%Qp, Cinr 0%nat, DecAgree v)]}) vl).
+  Proof.
+    revert l. induction vl as [|v vl IH]=> l FRESH.
+    - simpl. rewrite right_id. reflexivity.
+    - rewrite imap_cons. simpl. etrans. apply (IH (shift_loc l 1)).
+      { intros. by rewrite shift_loc_assoc. }
+      rewrite auth_frag_op assoc. apply cmra_update_op; last first.
+      { erewrite imap_ext. reflexivity. move=>i x/=. rewrite shift_loc_assoc.
+        f_equal. f_equal. lia. }
+      assert (Hinit: (to_heapVal (init_mem (shift_loc l 1) vl σ)) !! l = None).
+      { clear-FRESH. rewrite lookup_fmap fmap_None.
+        cut (0 < 1); last lia. generalize 1. revert l FRESH.
+        induction vl as [|v vl IH]=>/= l FRESH n Hn. by rewrite -(shift_loc_0 l).
+        rewrite shift_loc_assoc lookup_insert_ne;
+          [apply IH; auto; lia | destruct l; intros [=]; lia]. }
+      rewrite -[X in X ~~> _]right_id -{1}[to_heapVal (init_mem _ _ _)]left_id
+              shift_loc_0 /to_heapVal fmap_insert insert_singleton_op //.
+        by apply auth_update, alloc_unit_singleton_local_update.
+  Qed.
+
+  Lemma fresh_block_heap_free σ l heapFree:
+    (∀ m : Z, σ !! shift_loc l m = None) → heapFree_rel σ heapFree →
+    heapFree !! l.1 = None.
+  Proof.
+    intros FRESH REL. apply eq_None_not_Some; intros [[q s] [=[Hsne REL']%REL]].
+    destruct (map_choose s) as [i Hi%REL']; first done.
+    specialize (FRESH (i-l.2)). rewrite /shift_loc Zplus_minus in FRESH.
+    rewrite FRESH in Hi. by eapply is_Some_None.
+  Qed.
+
+  Lemma init_mem_update_free (l:loc) n heapFree σ:
+    (∀ m : Z, σ !! shift_loc l m = None) → heapFree_rel σ heapFree →
+    ● heapFree ~~>
+      ● ({[l.1 := (1%Qp, inter (l.2) n)]} ⋅ heapFree) ⋅
+      ◯ {[l.1 := (1%Qp, inter (l.2) n)]}.
+  Proof.
+    intros FRESH REL.
+    etrans; last apply auth_update, alloc_unit_singleton_local_update.
+    - rewrite right_id left_id. reflexivity.
+    - simpl. eauto using fresh_block_heap_free.
+    - split. done. apply inter_valid.
+  Qed.
+
+  Lemma init_mem_rel_free (l:loc) n heapFree vl σ:
+    0 < n → heapFree_rel σ heapFree →
+    (∀ m : Z, σ !! shift_loc l m = None) →
+    n = Datatypes.length vl →
+    heapFree_rel (init_mem l vl σ)
+                 ({[l.1 := (1%Qp, inter (l.2) (Z.to_nat n))]} ⋅ heapFree).
+  Proof.
+    intros Hn REL FRESH Hlen blk q s. destruct (decide (l.1 = blk)) as [EQ|NEQ].
+    - subst blk. rewrite lookup_op lookup_insert (fresh_block_heap_free σ)=>//.
+      intros [=]. subst. rewrite Nat2Z.id. split.
+      + destruct (List.length vl). lia. intros EQ%(f_equal (lookup (l.2))).
+        by rewrite lookup_insert lookup_empty in EQ.
+      + revert l FRESH. clear. induction vl as [|v vl IH]=>/=l FRESH i.
+        * specialize (FRESH (i-l.2)). rewrite /shift_loc Zplus_minus in FRESH.
+          rewrite lookup_empty FRESH. by split; intros []%is_Some_None.
+        * rewrite !lookup_insert_is_Some IH /=;
+                  last by intros; rewrite shift_loc_assoc.
+          destruct l. simpl. split; intros [|[]]; naive_solver congruence.
+    - rewrite lookup_op lookup_insert_ne // lookup_empty.
+      specialize (REL blk). revert REL. case: (heapFree !! blk); last done.
+      move=>? REL /REL [Hse Hs]. split. done. intros i. rewrite -Hs.
+      clear -NEQ. revert l NEQ. induction vl as [|v vl IH]=>//= l NEQ.
+      rewrite lookup_insert_is_Some IH //. naive_solver.
+  Qed.
+
+  Lemma wp_alloc N E (n:Z) Φ :
+    nclose N ⊆ E → 0 < n →
+    heap_ctx N ★
+    ▷ (∀ l vl, l ↦★ vl ★ n = length vl ★ †l…(Z.to_nat n) -★ Φ (LitV $ LitLoc l))
+    ⊢ WP Alloc (Lit $ LitInt n) @ E {{ Φ }}.
+  Proof.
+    iIntros {??} "[#Hinv HΦ]". rewrite /heap_ctx /heap_inv.
+    iInv> N as "INV". iDestruct "INV" as {σ heapFree} "(Hσ&Hvalσ&Hfree&%)".
+    iApply wp_pvs. iApply wp_alloc_pst =>//. iNext. iFrame "Hσ".
+    iIntros {l σ'} "(%&#Hσσ'&Hσ')". iDestruct "Hσσ'" as %(vl&HvlLen&Hvl).
+    iPvs (own_update _ (● to_heapVal σ) with "Hvalσ") as "[Hvalσ' Hmapsto]";
+      first apply (init_mem_update_val _ l vl); auto.
+    iPvs (own_update _ (● heapFree) with "Hfree") as "[Hfree' Hfreeable]";
+      first apply (init_mem_update_free l (Z.to_nat n) heapFree σ); auto.
+    iPvsIntro. iSplitL "Hσ' Hvalσ' Hfree'".
+    - iExists σ', _. subst σ'. iFrame. iPureIntro. by apply init_mem_rel_free.
+    - rewrite heap_freeable_eq /heap_freeable_def /auth_own. iApply "HΦ".
+      iFrame. iSplit; last auto. rewrite heap_mapsto_vec_auth /auth_own //.
+      destruct vl; simpl in *. lia. done.
+  Qed.
+
+End heap.
